@prefix owl: <http://www.w3.org/2002/07/owl#> .
@prefix rdf: <http://www.w3.org/1999/02/22-rdf-syntax-ns#> .
@prefix xml: <http://www.w3.org/XML/1998/namespace> .
@prefix xsd: <http://www.w3.org/2001/XMLSchema#> .
@prefix prov: <http://www.w3.org/ns/prov#> .
@prefix rdfs: <http://www.w3.org/2000/01/rdf-schema#> .
@prefix skos: <http://www.w3.org/2004/02/skos/core#> .
@base <http://www.w3.org/ns/prov#> .

<http://www.w3.org/TR/prov-dm/> rdf:type owl:Ontology ;
    rdfs:comment "Small subset of the prov-o ontology for use with records ontology" .

#################################################################
#    Annotation properties
#################################################################

###  http://www.w3.org/2004/02/skos/core#relatedProperty
skos:relatedProperty rdf:type owl:AnnotationProperty .


#################################################################
#    Object Properties
#################################################################

###  http://www.w3.org/ns/prov#hadMember
prov:hadMember rdf:type owl:ObjectProperty ;
               rdfs:domain prov:Collection ;
               rdfs:comment "A collection is an entity that provides a structure to some constituents, which are themselves entities. These constituents are said to be member of the collections." .


###  http://www.w3.org/ns/prov#wasDerivedFrom
prov:wasDerivedFrom rdf:type owl:ObjectProperty .


###  http://www.w3.org/ns/prov#wasRevisionOf
prov:wasRevisionOf rdf:type owl:ObjectProperty ;
                   rdfs:subPropertyOf prov:wasDerivedFrom .




#################################################################
#    Classes
#################################################################

###  http://www.w3.org/ns/prov#Collection
prov:Collection rdf:type owl:Class ;
                rdfs:subClassOf prov:Entity ;
                rdfs:comment "A collection is an entity that provides a structure to some constituents, which are themselves entities. These constituents are said to be member of the collections." ;
                rdfs:label "Collection" .


###  http://www.w3.org/ns/prov#Entity
prov:Entity rdf:type owl:Class ;
            rdfs:comment "An entity is a physical, digital, conceptual, or other kind of thing with some fixed aspects; entities may be real or imaginary." ;
            rdfs:label "Entity" .



###  Generated by the OWL API (version 4.5.9.2019-02-01T07:24:44Z) https://github.com/owlcs/owlapi
