@prefix dc: <http://purl.org/dc/elements/1.1/> .
@prefix owl: <http://www.w3.org/2002/07/owl#> .
@prefix rdf: <http://www.w3.org/1999/02/22-rdf-syntax-ns#> .
@prefix rec: <https://rdf.equinor.com/ontology/record/> .
@prefix xml: <http://www.w3.org/XML/1998/namespace> .
@prefix xsd: <http://www.w3.org/2001/XMLSchema#> .
@prefix prov: <http://www.w3.org/ns/prov#> .
@prefix rdfs: <http://www.w3.org/2000/01/rdf-schema#> .
@prefix skos: <http://www.w3.org/2004/02/skos/core#> .
@base <https://rdf.equinor.com/ontology/record/> .

<https://rdf.equinor.com/ontology/record-rules/> rdf:type owl:Ontology ;
                                            owl:imports <https://rdf.equinor.com/ontology/record-syntax/>;
                                            owl:versionIRI <https://rdf.equinor.com/ontology/record/2022-12-05> .

###  https://rdf.equinor.com/ontology/record/isInSubRecordTreeOf
rec:isInSubRecordTreeOf rdf:type owl:ObjectProperty ,
                                 owl:TransitiveProperty ;
                rdfs:domain rec:Record ;
                rdfs:range rec:Record ;
                rdfs:comment "This is the transitive closure of the relation rec:isSubRecordOf." .

###  https://rdf.equinor.com/ontology/record/isSubRecordOf
rec:isSubRecordOf rdfs:subPropertyOf rec:isInSubRecordTreeOf .

###  https://rdf.equinor.com/ontology/record/isInScopeInf
rec:isInScopeInf rdf:type owl:ObjectProperty ;
                 owl:propertyChainAxiom ( rec:isInSubRecordTreeOf
                                          rec:isInScope
                                        ) ;
                rdfs:domain rec:Record ;
                rdfs:comment "These are the scopes that a record inherits from its super-records, union with the explicit given scopes" .

###  https://rdf.equinor.com/ontology/record/replacesInf
rec:replacesInf rdf:type owl:ObjectProperty ,
                                owl:TransitiveProperty ;
                rdfs:subPropertyOf prov:wasRevisionOf ;
                rdfs:domain rec:Record ;
                rdfs:range rec:Record ;
                owl:propertyChainAxiom ( rec:isInSubRecordTreeOf
                                         rec:replaces
                                       ) ;
                rdfs:comment "This is the inferred replaces/derived from relation using subrecord and replaces relation" .
###  https://rdf.equinor.com/ontology/record/replaces
rec:replaces rdfs:subPropertyOf rec:replacesInf .