@prefix dc: <http://purl.org/dc/elements/1.1/> .
@prefix owl: <http://www.w3.org/2002/07/owl#> .
@prefix rdf: <http://www.w3.org/1999/02/22-rdf-syntax-ns#> .
@prefix rec: <https://rdf.equinor.com/ontology/record/> .
@prefix xml: <http://www.w3.org/XML/1998/namespace> .
@prefix xsd: <http://www.w3.org/2001/XMLSchema#> .
@prefix prov: <http://www.w3.org/ns/prov#> .
@prefix rdfs: <http://www.w3.org/2000/01/rdf-schema#> .
@prefix skos: <http://www.w3.org/2004/02/skos/core#> .
@base <https://rdf.equinor.com/ontology/record/> .

<https://rdf.equinor.com/ontology/record-rules/> rdf:type owl:Ontology ;
                                            rdfs:comment "This ontology does not make sense to apply to individual records, and does not give rules for individual records. Rather, the provenance from several records can be collected in a single graph, and then this ontology can be used on that graph to calculate head and scopes based on this. ";
                                            owl:imports <https://rdf.equinor.com/ontology/record-syntax/>;
                                            owl:versionIRI <https://rdf.equinor.com/ontology/record/2022-12-05> .

###  https://rdf.equinor.com/ontology/record/isInSubRecordTreeOf
rec:isInSubRecordTreeOf rdf:type owl:ObjectProperty ,
                                 owl:TransitiveProperty ;
                rdfs:subPropertyOf rec:hasNewerSuperRecordInf  ;
                rdfs:domain rec:Record ;
                rdfs:range rec:Record ;
                rdfs:comment "This is the transitive closure of the relation rec:isSubRecordOf." .

###  https://rdf.equinor.com/ontology/record/isSubRecordOf
rec:isSubRecordOf rdfs:subPropertyOf rec:isInSubRecordTreeOf .

###  https://rdf.equinor.com/ontology/record/isInScopeInf
rec:isInScopeInf rdf:type owl:ObjectProperty ;
                 owl:propertyChainAxiom ( rec:isInSubRecordTreeOf
                                          rec:isInScope
                                        ) ;
                rdfs:domain rec:Record ;
                rdfs:comment "These are the scopes that a record inherits from its super-records, union with the explicit given scopes" .

###  https://rdf.equinor.com/ontology/record/hasNewerSuperRecordInf
rec:hasNewerSuperRecordInf rdf:type owl:ObjectProperty ;
                rdfs:domain rec:Record ;
                rdfs:range rec:Record ;
                owl:propertyChainAxiom ( rec:isInSubRecordTreeOf
                                         rec:replacedBy
                                       ) ;
                rdfs:comment "These are all the super records which replaces the asserted super record." .

###  https://rdf.equinor.com/ontology/record/replacedBy
rec:replacedBy rdf:type owl:ObjectProperty ,
                       owl:TransitiveProperty ;
                rdfs:domain rec:Record ;
                rdfs:range rec:Record ;
                rdfs:comment "This is the transitive closure of the inverse relation rec:replaces." .

###  https://rdf.equinor.com/ontology/record/replaces
rec:replaces rdfs:subPropertyOf [ owl:inverseOf rec:replacedBy ] .

### https://rdf.equinor.com/ontology/record/hasRecordMember
rec:hasRecordMember rdf:type owl:ObjectProperty ;
               rdfs:subPropertyOf rec:hasMember ;
               rdfs:domain rec:Record ;
               rdfs:range rec:Record ;
               rdfs:label "has record member" ;
               rdfs:comment "A relation between a record and some other record." .

###  https://rdf.equinor.com/ontology/record/ReplacedRecord
rec:ReplacedRecord rdf:type owl:Class ;
                   rdfs:subClassOf rec:Record ;
                   owl:equivalentClass [ a owl:Restricton ;
                                           owl:onProperty rec:replacedBy ;
                                           owl:someValuesFrom rec:Record 
                                        ] ;
                    rdfs:comment "This is a record which has been replaced." .

###  https://rdf.equinor.com/ontology/record/NewestRecord
rec:NewestRecord rdf:type owl:Class ;
                   rdfs:subClassOf rec:Record ;
                   owl:equivalentClass [ a owl:Restricton ;
                                           owl:onProperty rec:replacedBy ;
                                           owl:maxCardinality 0 
                                        ] ;
                   owl:disjointWith rec:ReplacedRecord ;
                   rdfs:comment "This is a record which has not been replaced, and is therefore the newest." .