@prefix dc: <http://purl.org/dc/elements/1.1/> .
@prefix owl: <http://www.w3.org/2002/07/owl#> .
@prefix rdf: <http://www.w3.org/1999/02/22-rdf-syntax-ns#> .
@prefix rec: <https://rdf.equinor.com/ontology/record/> .
@prefix xml: <http://www.w3.org/XML/1998/namespace> .
@prefix xsd: <http://www.w3.org/2001/XMLSchema#> .
@prefix prov: <http://www.w3.org/ns/prov#> .
@prefix rdfs: <http://www.w3.org/2000/01/rdf-schema#> .
@prefix skos: <http://www.w3.org/2004/02/skos/core#> .
@base <https://rdf.equinor.com/ontology/record/> .

<https://rdf.equinor.com/ontology/record-syntax/> rdf:type owl:Ontology ;
                                            owl:versionIRI <https://rdf.equinor.com/ontology/record-syntax/2022-12-05> .

#################################################################
#    Annotation properties
#################################################################

###  http://www.w3.org/2004/02/skos/core#relatedProperty
skos:relatedProperty rdf:type owl:AnnotationProperty .


#################################################################
#    Object Properties
#################################################################

###  http://www.w3.org/ns/prov#hadMember
prov:hadMember rdf:type owl:ObjectProperty ;
               rdfs:domain prov:Collection ;
               rdfs:comment "A collection is an entity that provides a structure to some constituents, which are themselves entities. These constituents are said to be member of the collections." .


###  http://www.w3.org/ns/prov#wasDerivedFrom
prov:wasDerivedFrom rdf:type owl:ObjectProperty .


###  http://www.w3.org/ns/prov#wasRevisionOf
prov:wasRevisionOf rdf:type owl:ObjectProperty ;
                   rdfs:subPropertyOf prov:wasDerivedFrom .


###  https://rdf.equinor.com/ontology/record/describes
rec:describes rdf:type owl:ObjectProperty ;
              rdfs:domain rec:Record ;
              rdfs:comment "This relates a record to all the objects described in it. All IRIs desribed must occur in the content, and for any IRI occurring in the content/dataset, there must be a path between that IRI and one of the describes IRIs using only triples occurring in the content/dataset." ;
              rdfs:label "describes" ;
              rdfs:seeAlso <http://purl.obolibrary.org/obo/IAO_0000219> .

###  https://rdf.equinor.com/ontology/record/isInScope
rec:isInScope rdf:type owl:ObjectProperty ;
              rdfs:domain rec:Record ;
              rdfs:comment "Declares the scope in which the content of the record is valid. When there are several triples with the same subject the meaning is that the content is valid in the intersection of all the scopes. The scopes can be used to route the record to the correct storage and to regulate access. This relation propagates along the inverse of rec:isSubRecordOf" ;
              rdfs:label "is in scope" ;
              rdfs:seeAlso <http://purl.obolibrary.org/obo/IAO_0000142> .

###  https://rdf.equinor.com/ontology/record/isSubRecordOf
rec:isSubRecordOf rdf:type owl:ObjectProperty ;
                rdfs:subPropertyOf rec:isInSubRecordTreeOf ,
                [
                    owl:inverseOf prov:hadMember
                ] ;
                rdfs:domain rec:Record ;
                rdfs:range rec:Record ;
                rdfs:comment "A record can be a sub-record of another record. This does _not_ mean that the contents are related. Scopes are inherited from superrecord to subrecord, and subrecords are inherited via the replaces relation." .

###  https://rdf.equinor.com/ontology/record/replaces
rec:replaces rdf:type owl:ObjectProperty ;
             rdfs:subPropertyOf prov:wasRevisionOf ;
             rdfs:domain rec:Record ;
             rdfs:range rec:Record ;
             rdfs:comment "A record replaces the \"previous version\" of the record. The semantics is a full replace, that is, all the triples in the replaced version are removed and replaced by the present record. Note that subrecords are inherited from the replaced record" .

#################################################################
#    Classes
#################################################################

###  http://www.w3.org/ns/prov#Collection
prov:Collection rdf:type owl:Class ;
                rdfs:subClassOf prov:Entity ;
                rdfs:comment "A collection is an entity that provides a structure to some constituents, which are themselves entities. These constituents are said to be member of the collections." ;
                rdfs:label "Collection" .


###  http://www.w3.org/ns/prov#Entity
prov:Entity rdf:type owl:Class ;
            rdfs:comment "An entity is a physical, digital, conceptual, or other kind of thing with some fixed aspects; entities may be real or imaginary." ;
            rdfs:label "Entity" .


###  https://rdf.equinor.com/ontology/record/Record
rec:Record rdf:type owl:Class ;
           rdfs:subClassOf prov:Entity ;
           rdfs:comment "A record is an immutable named graph." ;
           rdfs:label "Record" ;
           rdfs:seeAlso <http://purl.obolibrary.org/obo/IAO_0000027> .


###  Generated by the OWL API (version 4.5.9.2019-02-01T07:24:44Z) https://github.com/owlcs/owlapi
