@prefix : <https://rdf.equinor.com/ontology/record-syntax/> .
@prefix dc: <http://purl.org/dc/elements/1.1/> .
@prefix owl: <http://www.w3.org/2002/07/owl#> .
@prefix rdf: <http://www.w3.org/1999/02/22-rdf-syntax-ns#> .
@prefix rec: <https://rdf.equinor.com/ontology/record/> .
@prefix xml: <http://www.w3.org/XML/1998/namespace> .
@prefix xsd: <http://www.w3.org/2001/XMLSchema#> .
@prefix prov: <http://www.w3.org/ns/prov#> .
@prefix rdfs: <http://www.w3.org/2000/01/rdf-schema#> .
@prefix skos: <http://www.w3.org/2004/02/skos/core#> .
@base <https://rdf.equinor.com/ontology/record/> .

<https://rdf.equinor.com/ontology/record-syntax/> rdf:type owl:Ontology ;
                                                   owl:versionIRI <https://rdf.equinor.com/ontology/record-syntax/2025-05-13> ;
                                                   owl:imports <http://www.w3.org/ns/prov-o>, <https://www.w3.org/TR/skos-reference/skos.rdf> .

#################################################################
#    Annotation properties
#################################################################

###  http://www.w3.org/2004/02/skos/core#relatedProperty
skos:relatedProperty rdf:type owl:AnnotationProperty .


#################################################################
#    Object Properties
#################################################################

###  https://rdf.equinor.com/ontology/record/describes
rec:describes rdf:type owl:ObjectProperty ;
              rdfs:domain rec:Record ;
              rdfs:comment "This relates a record to all the objects described in it. All IRIs desribed must occur in the content, and for any IRI occurring in the content/dataset, there must be a path between that IRI and one of the describes IRIs using only triples occurring in the content/dataset." ;
              rdfs:label "describes" ;
              rdfs:seeAlso <http://purl.obolibrary.org/obo/IAO_0000219> .


###  https://rdf.equinor.com/ontology/record/isInScope
rec:isInScope rdf:type owl:ObjectProperty ;
              rdfs:domain rec:Record ;
              rdfs:comment "Declares the scope in which the content of the record is valid. When there are several triples with the same subject the meaning is that the content is valid in the intersection of all the scopes. The scopes can be used to route the record to the correct storage and to regulate access. This relation propagates along rec:hasMember" ;
              rdfs:label "is in scope" ;
              rdfs:seeAlso <http://purl.obolibrary.org/obo/IAO_0000142> .

###  https://rdf.equinor.com/ontology/record/replaces
rec:replaces rdf:type owl:ObjectProperty ;
             rdfs:subPropertyOf prov:wasRevisionOf ;
             rdfs:domain rec:Record ;
             rdfs:range rec:Record ;
             rdfs:comment "A record replaces the \"previous version\" of the record. The semantics is a full replace, that is, all the triples in the replaced version are removed and replaced by the present record. Note that subrecords are inherited from the replaced record" .


### https://rdf.equinor.com/ontology/record/hasMember
rec:hasMember rdf:type owl:ObjectProperty ;
              rdfs:subPropertyOf prov:hadMember ;
              rdfs:domain rec:Record ;
              rdfs:comment "A relation between some record graph and some other named graph." .

### https://rdf.equinor.com/ontology/record/related
rec:related rdf:type owl:ObjectProperty ;
            rdfs:subPropertyOf skos:related ;
            rdfs:domain rec:Record ;
            rdfs:comment "A relation between a record and some IRI. These IRIs are related to the record in some undefined manner. The IRIs are used as a type of soft scoping." .

#################################################################
#    Classes
#################################################################

###  https://rdf.equinor.com/ontology/record/Record
rec:Record rdf:type owl:Class ;
           rdfs:subClassOf prov:Collection ;
           rdfs:comment "A record is an RDF dataset where there exists at least one named graph, the record metadata, which has other named graphs as its members." ;
           rdfs:label "Record" ;
           rdfs:seeAlso <http://purl.obolibrary.org/obo/IAO_0000027> .


###  Generated by the OWL API (version 4.5.26.2023-07-17T20:34:13Z) https://github.com/owlcs/owlapi
