@prefix : <https://rdf.equinor.com/ontology/record-syntax/> .
@prefix dc: <http://purl.org/dc/elements/1.1/> .
@prefix owl: <http://www.w3.org/2002/07/owl#> .
@prefix rdf: <http://www.w3.org/1999/02/22-rdf-syntax-ns#> .
@prefix rec: <https://rdf.equinor.com/ontology/record/> .
@prefix xml: <http://www.w3.org/XML/1998/namespace> .
@prefix xsd: <http://www.w3.org/2001/XMLSchema#> .
@prefix prov: <http://www.w3.org/ns/prov#> .
@prefix rdfs: <http://www.w3.org/2000/01/rdf-schema#> .
@prefix skos: <http://www.w3.org/2004/02/skos/core#> .
@base <https://rdf.equinor.com/ontology/record-syntax/> .

<https://rdf.equinor.com/ontology/record-syntax/> rdf:type owl:Ontology ;
                                                   owl:versionIRI <https://rdf.equinor.com/ontology/record-syntax/2025-05-13> ;
                                                   owl:imports <http://www.w3.org/2004/02/skos/core> ,
                                                               <http://www.w3.org/ns/prov-o> .

#################################################################
#    Annotation properties
#################################################################

###  http://www.w3.org/2004/02/skos/core#relatedProperty
skos:relatedProperty rdf:type owl:AnnotationProperty .


#################################################################
#    Object Properties
#################################################################

###  https://rdf.equinor.com/ontology/record/describes
rec:describes rdf:type owl:ObjectProperty ;
              rdfs:domain rec:Record ;
              rdfs:comment "This relates a record to all the objects described in its member graphs. All IRIs described must occur in some of the content, and for any IRI occurring in the content/dataset, there must be a path between that IRI and one of the describes IRIs using only triples occurring in the content/dataset." ;
              rdfs:label "describes" ;
              rdfs:seeAlso <http://purl.obolibrary.org/obo/IAO_0000219> .


###  https://rdf.equinor.com/ontology/record/hasMember
rec:hasMember rdf:type owl:ObjectProperty ;
              rdfs:subPropertyOf prov:hadMember ;
              rdfs:domain rec:Record ;
              rdfs:comment "A relation between some record and some other named graph. This means that the metadata available in the record is applicable to the member graph." ;
              rdfs:label "has member" .


###  https://rdf.equinor.com/ontology/record/isInScope
rec:isInScope rdf:type owl:ObjectProperty ;
              rdfs:domain rec:Record ;
              rdfs:comment "Declares the scope in which the content of the record is valid. When there are several triples with the same subject the meaning is that the content is valid in the intersection of all the scopes. The scopes can be used to route the record to the correct storage and to regulate access. This relation propagates along rec:hasMember" ;
              rdfs:label "is in scope" ;
              rdfs:seeAlso <http://purl.obolibrary.org/obo/IAO_0000142> .


###  https://rdf.equinor.com/ontology/record/related
rec:related rdf:type owl:ObjectProperty ;
            rdfs:subPropertyOf skos:related ;
            rdfs:domain rec:Record ;
            rdfs:comment "A relation between a record and some IRI. These IRIs are related to the record in some undefined manner. The IRIs are used as a type of soft scoping." ;
            rdfs:label "related" ;
            rdfs:seeAlso rec:isInScope .


###  https://rdf.equinor.com/ontology/record/replaces
rec:replaces rdf:type owl:ObjectProperty ;
             rdfs:subPropertyOf prov:wasRevisionOf ;
             rdfs:domain rec:Record ;
             rdfs:range rec:Record ;
             rdfs:label "replaces" ;
             rdfs:comment "A record replaces the \"previous version\" of the record. The semantics is a full replace, that is, all the triples in the replaced version are removed and replaced by the present record. Note that subrecords are inherited from the replaced record" .


#################################################################
#    Classes
#################################################################

###  https://rdf.equinor.com/ontology/record/BlankRecord
rec:BlankRecord rdf:type owl:Class ;
                rdfs:subClassOf prov:Collection ;
                rdfs:comment "A blank record has no real meaning on its own, it is up to any system implementing the type to determine how it is interpreted." ;
                rdfs:label "Blank record" .


###  https://rdf.equinor.com/ontology/record/DeletionRecord
rec:DeletionRecord rdf:type owl:Class ;
                   rdfs:subClassOf rec:BlankRecord ;
                   rdfs:comment "A deletion record has no members. This implies that there exists no information about the set of scopes and describes." ;
                   rdfs:label "Deletion record" .


###  https://rdf.equinor.com/ontology/record/Record
rec:Record rdf:type owl:Class ;
           rdfs:subClassOf rec:BlankRecord ;
           rdfs:comment "A record is an RDF dataset where there exists at least two named graphs. 1) The record metadata and 2) at least one other named graph as its member." ;
           rdfs:label "Record" ;
           rdfs:seeAlso <http://purl.obolibrary.org/obo/IAO_0000027> .


###  Generated by the OWL API (version 4.5.9.2019-02-01T07:24:44Z) https://github.com/owlcs/owlapi
