@prefix : <https://rdf.equinor.com/ontology/revision/> .
@prefix owl: <http://www.w3.org/2002/07/owl#> .
@prefix rdf: <http://www.w3.org/1999/02/22-rdf-syntax-ns#> .
@prefix xml: <http://www.w3.org/XML/1998/namespace> .
@prefix xsd: <http://www.w3.org/2001/XMLSchema#> .
@prefix rdfs: <http://www.w3.org/2000/01/rdf-schema#> .
@prefix skos: <http://www.w3.org/2004/02/skos/core#> .
@prefix prov: <http://www.w3.org/ns/prov#> .
@base <https://rdf.equinor.com/ontology/revision> .

<https://rdf.equinor.com/ontology/revision> rdf:type owl:Ontology ;
                                             owl:versionIRI <https://rdf.equinor.com/ontology/revision/v1.0> ;
                                             owl:imports <https://rdf.equinor.com/ontology/record-syntax/2022-12-05> .


#################################################################
#    Object Properties
#################################################################

###  https://rdf.equinor.com/ontology/revision/isNewRevisionOf
:isNewRevisionOf rdf:type owl:ObjectProperty ;
                rdfs:subPropertyOf <http://www.w3.org/ns/prov#wasDerivedFrom> ;
                rdfs:domain <https://rdf.equinor.com/ontology/revision/Revision> ;
                rdfs:range <https://rdf.equinor.com/ontology/revision/Revision> .

###  https://rdf.equinor.com/ontology/revision/hasAttachment
:hasAttachment rdf:type owl:ObjectProperty ;
                rdfs:subPropertyOf prov:hadMember ;
                rdfs:domain <https://rdf.equinor.com/ontology/revision/Document> ;
                rdfs:range <https://rdf.equinor.com/ontology/revision/Attachment> .

###  https://rdf.equinor.com/ontology/revision/describes
:describes rdf:type owl:ObjectProperty ;
                rdfs:domain <https://rdf.equinor.com/ontology/revision/Revision> .

###  https://rdf.equinor.com/ontology/revision/containsRecord
<https://rdf.equinor.com/ontology/revision/containsRecord> rdf:type owl:ObjectProperty ;
                                                         rdfs:subPropertyOf <http://www.w3.org/ns/prov#hadMember> ;
                                                         rdf:type owl:AsymmetricProperty ,
                                                                  owl:IrreflexiveProperty ;
                                                         rdfs:domain <https://rdf.equinor.com/ontology/revision/Revision> ;
                                                         rdfs:range <https://rdf.equinor.com/ontology/record/Record> ;
                                                         rdfs:comment "A revision contains one or more records. They represent the imutable state which the revision author(s) used for the revision process." .


#################################################################
#    Data properties
#################################################################

###  http://www.w3.org/ns/prov#generatedAtTime
<http://www.w3.org/ns/prov#generatedAtTime> rdf:type owl:DatatypeProperty ;
                                        rdfs:domain <http://www.w3.org/ns/prov#Entity> ;
                                        rdfs:range xsd:date ;
                                        rdfs:comment "Generation is the completion of production of a new entity by an activity. This entity did not exist before generation and becomes available for usage after this generation." .


###  https://rdf.equinor.com/ontology/revision/revisionNumber
:revisionNumber rdf:type owl:DatatypeProperty ;
                rdfs:domain <https://rdf.equinor.com/ontology/revision/DocumentRevision> ;
                rdfs:range xsd:string ;
                rdfs:comment "This name or number identifies the Revision in a series of Revisions." .


###  https://rdf.equinor.com/ontology/revision/issuedBy
:issuedBy rdf:type owl:DatatypeProperty ;
          rdfs:subPropertyOf prov:wasAttributedTo ;
          rdfs:domain <https://rdf.equinor.com/ontology/revision/DocumentRevision> ;
          rdfs:range xsd:string ;
          rdfs:comment "The author or responsible for the Revision" .


#################################################################
#    Classes
#################################################################

###  https://rdf.equinor.com/ontology/revision/DocumentRevision
<https://rdf.equinor.com/ontology/revision/DocumentRevision> rdf:type owl:Class ;
                                                            rdfs:subClassOf <https://rdf.equinor.com/ontology/revision/Revision> ;
                                                            owl:equivalentClass [ rdf:type owl:Restriction ;
                                                                                    owl:onProperty :describes ;
                                                                                    owl:someValuesFrom :Document
                                                            ] ;
                                                            rdfs:comment "A revision of a document is often calld a revision. It has an author and a issued by date." ;
                                                            rdfs:label "Document Revision" .

###  https://rdf.equinor.com/ontology/revision/Document
<https://rdf.equinor.com/ontology/revision/Document> rdf:type owl:Class ;
                                                                rdfs:subClassOf prov:Collection ;
                                                                rdfs:superClassOf [
                                                                    rdf:type owl:Restriction ;
                                                                    owl:onProperty [ owl:inverseOf :describes ];
                                                                    owl:someValuesFrom :DocumentRevision
                                                                ];
                                                                rdfs:comment "A document is a named collection of files with a purpose." ;
                                                                rdfs:label "Document" .

###  https://rdf.equinor.com/ontology/revision/Attachment
<https://rdf.equinor.com/ontology/revision/Attachment> rdf:type owl:Class ;
                                                                rdfs:subClassOf prov:Entity ;
                                                                rdfs:comment "An attachment is a physical file, for example an excel file. It is " ;
                                                                rdfs:label "Attachment" .

###  https://rdf.equinor.com/ontology/revision/Revision
<https://rdf.equinor.com/ontology/revision/Revision> rdf:type owl:Class ;
                                                        rdfs:subClassOf <http://www.w3.org/ns/prov#Collection> ;
                                                        rdfs:comment "A revision is a collection of records. It can also point to the previous Revision." ;
                                                        rdfs:label "Revision" .


###  Generated by the OWL API (version 4.5.9.2019-02-01T07:24:44Z) https://github.com/owlcs/owlapi
