@prefix : <https://rdf.equinor.com/ontology/revision/> .
@prefix owl: <http://www.w3.org/2002/07/owl#> .
@prefix rdf: <http://www.w3.org/1999/02/22-rdf-syntax-ns#> .
@prefix xml: <http://www.w3.org/XML/1998/namespace> .
@prefix xsd: <http://www.w3.org/2001/XMLSchema#> .
@prefix prov: <http://www.w3.org/ns/prov> .
@prefix rdfs: <http://www.w3.org/2000/01/rdf-schema#> .
@prefix skos: <http://www.w3.org/2004/02/skos/core#> .
@prefix prov: <http://www.w3.org/ns/prov#> .
@base <https://rdf.equinor.com/ontology/revision> .

<https://rdf.equinor.com/ontology/revision> rdf:type owl:Ontology ;
                                             owl:versionIRI <https://rdf.equinor.com/ontology/revision/2023-01-10> ;
                                             owl:imports <https://rdf.equinor.com/ontology/record-syntax/2022-12-05> .

#################################################################
#    Annotation properties
#################################################################

###  http://www.w3.org/2004/02/skos/core#prefLabel
skos:prefLabel rdf:type owl:AnnotationProperty .


#################################################################
#    Datatypes
#################################################################

###  http://www.w3.org/2001/XMLSchema#date
xsd:date rdf:type rdfs:Datatype .


#################################################################
#    Object Properties
#################################################################

###  http://www.w3.org/ns/prov#used
<http://www.w3.org/ns/prov#used> rdf:type owl:ObjectProperty ;
                                 rdfs:domain <http://www.w3.org/ns/prov#Activity> ;
                                 rdfs:range <http://www.w3.org/ns/prov#Entity> ;
                                 rdfs:comment "Usage is the beginning of utilizing an entity by an activity. Before usage, the activity had not begun to utilize this entity and could not have been affected by the entity." .


###  https://rdf.equinor.com/ontology/revision/isNewRevisionOf
:isNewRevisionOf rdf:type owl:ObjectProperty ;
                rdfs:subPropertyOf <http://www.w3.org/ns/prov#wasDerivedFrom> ;
                rdfs:domain <https://rdf.equinor.com/ontology/revision/Revision> ;
                rdfs:range <https://rdf.equinor.com/ontology/revision/Revision> .


###  https://rdf.equinor.com/ontology/revision/contains
<https://rdf.equinor.com/ontology/revision/contains> rdf:type owl:ObjectProperty ;
                                                         rdfs:subPropertyOf <http://www.w3.org/ns/prov#hadMember> ;
                                                         rdf:type owl:AsymmetricProperty ,
                                                                  owl:IrreflexiveProperty ;
                                                         rdfs:domain <https://rdf.equinor.com/ontology/revision/Revision> ;
                                                         rdfs:range <https://rdf.equinor.com/ontology/record/Record> ;
                                                         rdfs:comment "A revision contains one or more records. They represent the imutable state which the revision author(s) used for the revision process." .


#################################################################
#    Data properties
#################################################################

###  http://www.w3.org/ns/prov#endedAtTime
<http://www.w3.org/ns/prov#endedAtTime> rdf:type owl:DatatypeProperty ;
                                        rdfs:domain <http://www.w3.org/ns/prov#Activity> ;
                                        rdfs:range xsd:dateTime ;
                                        rdfs:comment "End is when an activity is deemed to have been ended by an entity, known as trigger. The activity no longer exists after its end. Any usage, generation, or invalidation involving an activity precedes the activity's end. An end may refer to a trigger entity that terminated the activity, or to an activity, known as ender that generated the trigger." .


###  http://www.w3.org/ns/prov#generatedAtTime
<http://www.w3.org/ns/prov#generatedAtTime> rdf:type owl:DatatypeProperty ;
                                        rdfs:domain <http://www.w3.org/ns/prov#Entity> ;
                                        rdfs:range xsd:date ;
                                        rdfs:comment "Generation is the completion of production of a new entity by an activity. This entity did not exist before generation and becomes available for usage after this generation." .


###  https://rdf.equinor.com/ontology/revision/revisionNumber
:revisionNumber rdf:type owl:DatatypeProperty ;
                rdfs:domain <https://rdf.equinor.com/ontology/revision/DocumentRevision> ;
                rdfs:range xsd:string ;
                rdfs:comment "This name or number identifies the Revision in a series of Revisions." .


###  https://rdf.equinor.com/ontology/revision/issuedBy
:issuedBy rdf:type owl:DatatypeProperty ;
          rdfs:subPropertyOf prov:wasAttributedTo ;
          rdfs:domain <https://rdf.equinor.com/ontology/revision/DocumentRevision> ;
          rdfs:range xsd:string ;
          rdfs:comment "The author or responsible for the Revision" .


#################################################################
#    Classes
#################################################################

###  http://www.w3.org/ns/prov#Activity
<http://www.w3.org/ns/prov#Activity> rdf:type owl:Class ;
                                     owl:disjointWith <http://www.w3.org/ns/prov#Entity> ;
                                     rdfs:comment "An activity is something that occurs over a period of time and acts upon or with entities; it may include consuming, processing, transforming, modifying, relocating, using, or generating entities." ;
                                     rdfs:label "Activity" .


###  http://www.w3.org/ns/prov#Entity

###  https://rdf.equinor.com/ontology/revision/DocumentRevision
<https://rdf.equinor.com/ontology/revision/DocumentRevision> rdf:type owl:Class ;
                                                                rdfs:subClassOf <https://rdf.equinor.com/ontology/revision/Revision> ;
                                                                rdfs:comment "A revision of a document is often calld a revision. It has an author and a issued by date." ;
                                                                rdfs:label "Document Revision" .


###  https://rdf.equinor.com/ontology/revision/Revision
<https://rdf.equinor.com/ontology/revision/Revision> rdf:type owl:Class ;
                                                        rdfs:subClassOf <http://www.w3.org/ns/prov#Collection> ;
                                                        rdfs:comment "A revision is a collection of records. It can also point to the previous Revision." ;
                                                        rdfs:label "Revision" .


###  Generated by the OWL API (version 4.5.9.2019-02-01T07:24:44Z) https://github.com/owlcs/owlapi
