@prefix : <https://rdf.equinor.com/ontology/revision/> .
@prefix owl: <http://www.w3.org/2002/07/owl#> .
@prefix rdf: <http://www.w3.org/1999/02/22-rdf-syntax-ns#> .
@prefix xml: <http://www.w3.org/XML/1998/namespace> .
@prefix xsd: <http://www.w3.org/2001/XMLSchema#> .
@prefix prov: <http://www.w3.org/ns/prov#> .
@prefix rdfs: <http://www.w3.org/2000/01/rdf-schema#> .
@prefix skos: <http://www.w3.org/2004/02/skos/core#> .
@base <https://rdf.equinor.com/ontology/revision> .

<https://rdf.equinor.com/ontology/revision> rdf:type owl:Ontology ;
                                             owl:versionIRI :v1.0 ;
                                             owl:imports <https://rdf.equinor.com/ontology/record-syntax/2022-12-05> .

#################################################################
#    Datatypes
#################################################################

###  http://www.w3.org/2001/XMLSchema#date
xsd:date rdf:type rdfs:Datatype .


#################################################################
#    Object Properties
#################################################################

###  https://rdf.equinor.com/ontology/revision/containsRecord
:containsRecord rdf:type owl:ObjectProperty ;
                rdfs:subPropertyOf prov:hadMember ;
                rdf:type owl:AsymmetricProperty ,
                         owl:IrreflexiveProperty ;
                rdfs:domain :Revision ;
                rdfs:range <https://rdf.equinor.com/ontology/record/Record> ;
                rdfs:comment "A revision contains one or more records. They represent the imutable state which the revision author(s) used for the revision process." .


###  http://www.w3.org/ns/prov#wasAssociatedWith
prov:wasAssociatedWith rdf:type owl:ObjectProperty ;
                                            rdfs:subPropertyOf owl:topObjectProperty ;
                                            rdfs:comment "Attribution is the ascribing of an entity to an agent." ,
                                                         "comment responsible" ;
                                            rdfs:label "was associated with" .


###  https://rdf.equinor.com/ontology/revision/describes
:describes rdf:type owl:ObjectProperty ;
           rdfs:domain :Revision ;
           rdfs:comment "Relates a revision to a document or object it is a revision of or describes." .


###  https://rdf.equinor.com/ontology/revision/isNewRevisionOf
:isNewRevisionOf rdf:type owl:ObjectProperty ;
                 rdfs:subPropertyOf prov:wasDerivedFrom ;
                 rdfs:domain :Revision ;
                 rdfs:range :Revision .


#################################################################
#    Data properties
#################################################################

###  http://www.w3.org/ns/prov#generatedAtTime
prov:generatedAtTime rdf:type owl:DatatypeProperty ;
                     rdfs:domain prov:Entity ;
                     rdfs:range xsd:date ;
                     rdfs:comment "Generation is the completion of production of a new entity by an activity. This entity did not exist before generation and becomes available for usage after this generation." .


###  http://www.w3.org/ns/prov#wasAttributedTo
prov:wasAttributedTo rdf:type owl:DatatypeProperty ;
                    rdfs:domain prov:Entity ;
                    rdfs:comment "Attribution is the ascribing of an entity to an agent." .


###  https://rdf.equinor.com/ontology/revision/issuedBy
:issuedBy rdf:type owl:DatatypeProperty ;
          rdfs:subPropertyOf prov:wasAttributedTo ;
          rdfs:domain :DocumentRevision ;
          rdfs:range xsd:string ;
          rdfs:comment "The author or responsible for the Revision" .


###  https://rdf.equinor.com/ontology/revision/revisionNumber
:revisionNumber rdf:type owl:DatatypeProperty ;
                rdfs:domain :DocumentRevision ;
                rdfs:range xsd:string ;
                rdfs:comment "This name or number identifies the Revision in a series of Revisions." .

###  https://rdf.equinor.com/ontology/revision/hasSequenceNumber
:hasSequenceNumber rdf:type owl:DatatypeProperty ;
                   rdfs:range xsd:int ;
                   rdfs:comment "The position of this revision in a natural number sequence." ;
                   rdfs:label "Revision Sequence Number" .

#################################################################
#    Classes
#################################################################

###  https://rdf.equinor.com/ontology/revision/DocumentRevision
:DocumentRevision rdf:type owl:Class ;
                  rdfs:subClassOf :Revision ;
                  rdfs:comment "A revision of a document is some published edition or version or the documnet which the producer gives a special status. It has an author and a issued by date." ;
                  rdfs:label "Document Revision" .


###  https://rdf.equinor.com/ontology/revision/Revision
:Revision rdf:type owl:Class ;
          rdfs:subClassOf prov:Collection ;
          rdfs:comment "A revision is a collection of records. It can also point to the previous Revision." ;
          rdfs:label "Revision" .



###  Generated by the OWL API (version 4.5.9.2019-02-01T07:24:44Z) https://github.com/owlcs/owlapi
