@prefix : <https://rdf.equinor.com/ontology/revision#> .
@prefix owl: <http://www.w3.org/2002/07/owl#> .
@prefix rdf: <http://www.w3.org/1999/02/22-rdf-syntax-ns#> .
@prefix xml: <http://www.w3.org/XML/1998/namespace> .
@prefix xsd: <http://www.w3.org/2001/XMLSchema#> .
@prefix prov: <http://www.w3.org/ns/prov> .
@prefix rdfs: <http://www.w3.org/2000/01/rdf-schema#> .
@base <https://rdf.equinor.com/ontology/revision> .

<https://rdf.equinor.com/ontology/revision> rdf:type owl:Ontology ;
                                             owl:versionIRI <https://rdf.equinor.com/ontology/revision/2023-01-10> ;
                                             owl:imports <https://rdf.equinor.com/ontology/record-syntax/2022-12-05> .

#################################################################
#    Object Properties
#################################################################

###  http://purl.org/stuff/rev#revises
<http://purl.org/stuff/rev#revises> rdf:type owl:ObjectProperty ;
                                    rdfs:subPropertyOf <http://www.w3.org/ns/prov#used> ;
                                    rdf:type owl:AsymmetricProperty ,
                                             owl:IrreflexiveProperty ;
                                    rdfs:domain <http://purl.org/stuff/rev#Revision> ;
                                    rdfs:range <https://rdf.equinor.com/ontology/record/Record> ;
                                    rdfs:comment "A revision revises a non-empty collection of records. They represent the imutable state which the revision author(s) used for the revision process." .


###  http://www.w3.org/ns/prov#used
<http://www.w3.org/ns/prov#used> rdf:type owl:ObjectProperty ;
                                 rdfs:domain <http://www.w3.org/ns/prov#Activity> ;
                                 rdfs:range <http://www.w3.org/ns/prov#Entity> ;
                                 rdfs:comment "Usage is the beginning of utilizing an entity by an activity. Before usage, the activity had not begun to utilize this entity and could not have been affected by the entity." .


#################################################################
#    Data properties
#################################################################

###  http://purl.org/stuff/rev#revisedAtDate
<http://purl.org/stuff/rev#revisedAtDate> rdf:type owl:DatatypeProperty ;
                                          rdfs:subPropertyOf <http://www.w3.org/ns/prov#endedAtTime> ;
                                          rdfs:comment "A revision is associated with the date or time at which the revision was made" .


###  http://purl.org/stuff/rev#wasRevisedBy
<http://purl.org/stuff/rev#wasRevisedBy> rdf:type owl:DatatypeProperty ;
                                         rdfs:domain <http://purl.org/stuff/rev#Revision> ;
                                         rdfs:range xsd:string ;
                                         rdfs:comment "The name(s) of the revisor(s)" .


###  http://www.w3.org/ns/prov#endedAtTime
<http://www.w3.org/ns/prov#endedAtTime> rdf:type owl:DatatypeProperty ;
                                        rdfs:domain <http://www.w3.org/ns/prov#Activity> ;
                                        rdfs:range xsd:dateTime ;
                                        rdfs:comment "End is when an activity is deemed to have been ended by an entity, known as trigger. The activity no longer exists after its end. Any usage, generation, or invalidation involving an activity precedes the activity's end. An end may refer to a trigger entity that terminated the activity, or to an activity, known as ender that generated the trigger." .


#################################################################
#    Classes
#################################################################

###  http://purl.org/stuff/rev#Revision
<http://purl.org/stuff/rev#Revision> rdf:type owl:Class ;
                                     rdfs:subClassOf <http://www.w3.org/ns/prov#Activity> ,
                                                     [ rdf:type owl:Restriction ;
                                                       owl:onProperty <http://purl.org/stuff/rev#revises> ;
                                                       owl:someValuesFrom <https://rdf.equinor.com/ontology/record/Record>
                                                     ] ,
                                                     [ rdf:type owl:Restriction ;
                                                       owl:onProperty <http://purl.org/stuff/rev#revises> ;
                                                       owl:allValuesFrom <https://rdf.equinor.com/ontology/record/Record>
                                                     ] ;
                                     rdfs:comment "A business revision is the activity of stating that several records together have a certain property. A revision has a date, author and at least one revises relation." ;
                                     rdfs:label "Revision" .


###  http://www.w3.org/ns/prov#Activity
<http://www.w3.org/ns/prov#Activity> rdf:type owl:Class ;
                                     owl:disjointWith <http://www.w3.org/ns/prov#Entity> ;
                                     rdfs:comment "An activity is something that occurs over a period of time and acts upon or with entities; it may include consuming, processing, transforming, modifying, relocating, using, or generating entities." ;
                                     rdfs:label "Activity" .


###  http://www.w3.org/ns/prov#Entity

###  Generated by the OWL API (version 4.5.9.2019-02-01T07:24:44Z) https://github.com/owlcs/owlapi
